1446. Consecutive Characters

Given a string `s`, the power of the string is the maximum length of a non-empty substring that contains only one unique character.

Return the power of the string.

 

**Example 1:**
```
Input: s = "leetcode"
Output: 2
Explanation: The substring "ee" is of length 2 with the character 'e' only.
```

**Example 2:**
```
Input: s = "abbcccddddeeeeedcba"
Output: 5
Explanation: The substring "eeeee" is of length 5 with the character 'e' only.
```

**Example 3:**
```
Input: s = "triplepillooooow"
Output: 5
```

**Example 4:**
```
Input: s = "hooraaaaaaaaaaay"
Output: 11
```

**Example 5:**
```
Input: s = "tourist"
Output: 1
```

**Constraints:**

* `1 <= s.length <= 500`
* `s` contains only lowercase English letters.

# Submissions
---
**Solution 1: (One Pass)**
```
Runtime: 48 ms
Memory Usage: 14.1 MB
```
```python
class Solution:
    def maxPower(self, s: str) -> int:
        count = 0
        max_count = 0
        previous = None
        for c in s:
            if c == previous:
                # if same as previous one, increase the count
                count += 1
            else:
                # else, reset the count
                previous = c
                count = 1
            max_count = max(max_count, count)
        return max_count
```

**Solution 2: (itertools)**
```
Runtime: 96 ms
Memory Usage: 13.9 MB
```
```python
class Solution:
    def maxPower(self, s: str) -> int:
        return max(len(list(g)) for k, g in itertools.groupby(s))
```

**Solution 3: (Greedy)**
```
Runtime: 68 ms
Memory Usage: 13.9 MB
```
```python
class Solution:
    def maxPower(self, s: str) -> int:
        ans = cnt = 1
        for i in range(1, len(s)):
            if s[i] == s[i - 1]:
                cnt += 1
            else:
                cnt = 1
            ans = max(ans,cnt)        
        return ans
```

**Solution 4: (Greedy)**
```
Runtime: 0 ms
Memory Usage: 5.8 MB
```
```c
int maxPower(char * s){
    int i = 0, j = 0, ans = 0;
    while (s[j]) {
        if (s[j] != s[i]) {
            i = j;
        }
        ans = (ans > j-i+1 ? ans : j-i+1);
        j += 1;
    }
    return ans;
}
```
